rt refine: The state relation is not empty.
Defined a series of `zeroed` states on the abstract and haskell sides
that together satisfy the state relation. These states do not satisfy
invs or invs', that would be a little more work.

Signed-off-by: Mitchell Buckley <mitchell.buckley@data61.csiro.au>

proof/refine/ARM/KHeap_R.thy
@@ -3311,5 +3311,98 @@ lemma refillSufficient_wp:
   apply (wpsimp wp: getRefills_wp)
   by (clarsimp simp: sufficientRefills_def obj_at'_def)
 
+definition
+  "zeroed_arch_abstract_state \<equiv> \<lparr>
+    arm_asid_table = Map.empty,
+    arm_hwasid_table = Map.empty,
+    arm_next_asid = 0,
+    arm_asid_map = Map.empty,
+    arm_global_pd = 0,
+    arm_global_pts = [],
+    arm_kernel_vspace = K ArmVSpaceUserRegion
+  \<rparr>"
+
+definition
+  "zeroed_abstract_state \<equiv>
+  \<lparr>kheap = Map.empty,
+  cdt = Map.empty,
+  is_original_cap = (K True),
+  cur_thread = 0,
+  idle_thread = 0,
+  consumed_time = 0,
+  cur_time = 0,
+  cur_sc = 0,
+  reprogram_timer = True,
+  scheduler_action = resume_cur_thread,
+  domain_list = [],
+  domain_index = 0,
+  cur_domain = 0,
+  domain_time = 0,
+  ready_queues = (\<lambda>_ _. []),
+  release_queue = [],
+  machine_state = init_machine_state,
+  interrupt_irq_node = (\<lambda>irq. ucast irq << cte_level_bits),
+  interrupt_states = (K irq_state.IRQInactive),
+  arch_state = zeroed_arch_abstract_state\<rparr> :: abstract_state"
+
+definition zeroed_extended_state :: det_ext where
+  "zeroed_extended_state \<equiv>
+   \<lparr>work_units_completed_internal = 0,
+    cdt_list_internal = K []\<rparr>"
+
+definition zeroed_det_state :: det_state where
+  "zeroed_det_state \<equiv> abstract_state.extend zeroed_abstract_state (state.fields zeroed_extended_state)"
+
+definition
+ "zeroed_arch_kernel_state \<equiv> ARMKernelState Map.empty Map.empty 0 Map.empty 0 [] (K ArmVSpaceUserRegion)"
+
+definition
+ "zeroed_kernel_state \<equiv>
+ \<lparr>ksPSpace = Map.empty,
+  gsUserPages = Map.empty,
+  gsCNodes = Map.empty,
+  gsUntypedZeroRanges = {},
+  gsMaxObjectSize = 0,
+  ksDomScheduleIdx = 0,
+  ksDomSchedule = [],
+  ksCurDomain = 0,
+  ksDomainTime = 0,
+  ksReadyQueues = K [],
+  ksReleaseQueue = [],
+  ksReadyQueuesL1Bitmap = K 0,
+  ksReadyQueuesL2Bitmap = K 0,
+  ksCurThread = 0,
+  ksIdleThread = 0,
+  ksConsumedTime = 0,
+  ksCurTime = 0,
+  ksCurSc = 0,
+  ksReprogramTimer = True,
+  ksSchedulerAction = ResumeCurrentThread,
+  ksInterruptState = (InterruptState 0 (K IRQInactive)),
+  ksWorkUnitsCompleted = 0,
+  ksArchState = zeroed_arch_kernel_state,
+  ksMachineState = init_machine_state\<rparr>"
+
+lemmas zeroed_state_defs = zeroed_det_state_def zeroed_abstract_state_def
+                           zeroed_arch_abstract_state_def zeroed_extended_state_def
+                           zeroed_kernel_state_def abstract_state.defs zeroed_arch_kernel_state_def
+
+lemma non_empty_refine_state_relation:
+  "(zeroed_det_state, zeroed_kernel_state) \<in> state_relation"
+  apply (clarsimp simp: state_relation_def zeroed_state_defs
+                        state.defs)
+  apply (intro conjI)
+           apply (clarsimp simp: pspace_relation_def pspace_dom_def)
+          apply (clarsimp simp: sc_replies_relation_def vs_all_heap_simps)
+         apply (clarsimp simp: ready_queues_relation_def)
+        apply (clarsimp simp: release_queue_relation_def)
+       apply (clarsimp simp: ghost_relation_def)
+      apply (fastforce simp: cdt_relation_def swp_def dest: cte_wp_at_domI)
+     apply (clarsimp simp: cdt_list_relation_def map_to_ctes_def)
+    apply (clarsimp simp: revokable_relation_def map_to_ctes_def)
+   apply (clarsimp simp: zeroed_state_defs arch_state_relation_def)
+  apply (clarsimp simp: interrupt_state_relation_def irq_state_relation_def cte_level_bits_def)
+  done
+
 end
 end
